# Thinking

<pre>

65	64	63	62	61	60	59	58	57
66	37	36	35	34	33	32	31	56
67	38	17	16	15	14	13	30	55
68	39	18	5	4	3	12	29	54
69	40	19	6	1	2	11	28	53
70	41	20	7	8	9	10	27	52
71	42	21	22	23	24	25	26	51
72	43	44	45	46	47	48	49	50
73	74	75	76	77	78	79	80	81

0	1	2	3	4  (n)

1	2	11	28	53
  1    9   17  25
(-1) -> C
  0    8   16  24

1	4	15	34	61
  3   11   19  27
(-3) -> C
  0    8   16  24



l<sub>n</sub> = l<sub>n-1</sub> + (n-1)*8 + C

l<sub>3</sub> = 11 + 2*8 + 1
   = 11 + 16 + 1
   = 28

l<sub>3</sub> = 15 + 2*8 + 3
   = 15 + 16 + 3
   = 34


l<sub>0</sub> = 1
l<sub>1</sub> = 1 + C
l<sub>2</sub> = (1 + C) + 1*8 + C
   = 1 + 2C + 1*8
l<sub>3</sub> = (1 + 2C + 1*8) + 2*8 + C
   = 1 + 3C + 3*8
l<sub>4</sub> = (1 + 3C + 3*8) + 3*8 + C
   = 1 + 4C + 6*8
l<sub>5</sub> = (1 + 4C + 6*8) + 4*8 + C
   = 1 + 5C + 10*8
l<sub>6</sub> = (1 + 5C + 10*8) + 5*8 + C
   = 1 + 6C + 15*8

1 + n*C + ?*8

n:   0  1  2  3  4  5   6
?:   0  0  1  3  6  10  15 <- triangle numbers (n-1) T
n-1: -1 0  1  2  3  4   5

l<sub>n</sub> = 1 + n*C + (T<sub>n-1</sub> * 8)

</pre>
